Main2.fst mostly clean, fix extraction
still a few verif issues

src/Main2.fst
@@ -180,8 +180,13 @@ let slab_free' (i:US.t{US.v i < US.v nb_size_classes * US.v nb_arenas}) (ptr: ar
     let diff' = offset (ptr_of ptr) - offset (ptr_of sc.data.slab_region) in
     same_base_array ptr sc.data.slab_region /\
     0 <= diff' /\
-    diff' < US.v slab_size /\
-    (diff' % U32.v page_size) % U32.v (get_u32 sc.data.size) == 0 /\
+    (sc.data.is_extended ==>
+      diff' % US.v sc_ex_slab_size == 0
+    ) /\
+    (not sc.data.is_extended ==>
+      (diff' % U32.v page_size) % U32.v (get_u32 sc.data.size) == 0
+    ) /\
+    diff' < US.v sc_slab_region_size /\
     A.length ptr == U32.v (get_u32 sc.data.size) /\
     US.v diff = diff'
   ))
@@ -212,59 +217,60 @@ let slab_free' (i:US.t{US.v i < US.v nb_size_classes * US.v nb_arenas}) (ptr: ar
 /// entire memory provided by the allocator:
 /// If a pointer is within a size class and aligned with
 /// the slots, then its length corresponds to the slot size
-let within_size_class_i (ptr:A.array U8.t) (sc: size_class_struct) : prop = (
-  // If ptr is within the size class sc
-  same_base_array sc.slab_region ptr /\
-  A.offset (A.ptr_of ptr) - A.offset (A.ptr_of (G.reveal sc.slab_region)) >= 0 /\
-  A.offset (A.ptr_of ptr) - A.offset (A.ptr_of (G.reveal sc.slab_region)) < US.v slab_size /\
-  // and it is aligned on the slots
-  ((A.offset (A.ptr_of ptr) - A.offset (A.ptr_of (G.reveal sc.slab_region))) % U32.v page_size) % U32.v (get_u32 sc.size) = 0) ==>
+let within_size_class_i (ptr:A.array U8.t) (sc: size_class_struct) : prop =
+  (
+    let diff = A.offset (A.ptr_of ptr) - A.offset (A.ptr_of (G.reveal sc.slab_region)) in
+    // If ptr is within the size class sc
+    same_base_array sc.slab_region ptr /\
+    0 <= diff /\
+    diff < US.v sc_slab_region_size /\
+    // and it is aligned on the slots
+    (sc.is_extended ==>
+      diff % US.v sc_ex_slab_size == 0
+    ) /\
+    (not sc.is_extended ==>
+      (diff % U32.v page_size) % U32.v (get_u32 sc.size) == 0
+    )
+  ) ==>
     // then its length is the length of a slot
     A.length ptr == U32.v (get_u32 sc.size)
 
-#push-options "--fuel 0 --ifuel 1 --z3rlimit 150"
+#restart-solver
+
+#push-options "--fuel 0 --ifuel 1 --z3rlimit 150 --quake 10/10"
 /// Elimination lemma for `within_size_class_i`, triggering F* to prove the precondition
 /// of the implication
-let elim_within_size_class_i (ptr:A.array U8.t) (i:nat{i < Seq.length sc_all.g_size_classes}) (size:sc)
+let elim_within_size_class_i
+  (ptr:A.array U8.t)
+  (i:nat{i < Seq.length sc_all.g_size_classes})
+  (size:U32.t)
   : Lemma
   (requires (
     let sc : size_class = G.reveal (Seq.index sc_all.g_size_classes i) in
-    size == get_u32 sc.data.size /\
+    let diff = A.offset (A.ptr_of ptr) - A.offset (A.ptr_of (G.reveal sc.data.slab_region)) in
     within_size_class_i ptr sc.data /\
+    size == get_u32 sc.data.size /\
     same_base_array sc.data.slab_region ptr /\
-    A.offset (A.ptr_of ptr) - A.offset (ptr_of (G.reveal sc.data.slab_region)) >= 0 /\
-    A.offset (A.ptr_of ptr) - A.offset (ptr_of (G.reveal sc.data.slab_region)) < US.v slab_size /\
-    ((A.offset (A.ptr_of ptr) - A.offset (ptr_of (G.reveal sc_all.slab_region))) % U32.v page_size) % U32.v size = 0))
+    0 <= diff /\
+    diff < US.v sc_slab_region_size /\
+    (sc.data.is_extended ==>
+      diff % US.v sc_ex_slab_size == 0
+    ) /\
+    (not sc.data.is_extended ==>
+      (diff % U32.v page_size) % U32.v (get_u32 sc.data.size) == 0
+    )
+  ))
   (ensures (
     let sc : size_class = G.reveal (Seq.index sc_all.g_size_classes i) in
-    ((A.offset (A.ptr_of ptr) - A.offset (ptr_of (G.reveal sc.data.slab_region))) % U32.v page_size) % U32.v size = 0 /\
     A.length ptr == U32.v size
   ))
   =
-  let sc : size_class = G.reveal (Seq.index sc_all.g_size_classes i) in
-  let off_ptr = A.offset (A.ptr_of ptr) in
-  let off1 = A.offset (A.ptr_of (G.reveal sc_all.slab_region)) in
-  let off2 = A.offset (A.ptr_of (G.reveal sc.data.slab_region)) in
-  admit ();
-  assert (off2 - off1 = i * US.v slab_size);
-  assert (off_ptr - off1 = off_ptr - off2 + i * US.v slab_size);
-  assert (i * US.v slab_size == i * US.v metadata_max * U32.v page_size);
-  Math.Lemmas.lemma_mod_plus
-    (off_ptr - off2)
-    (i * US.v metadata_max)
-    (U32.v page_size);
-  assert (
-    (off_ptr - off1) % U32.v page_size
-    ==
-    (off_ptr - off2) % U32.v page_size
-  )
+  ()
 #pop-options
 
 let within_size_classes_pred (ptr:A.array U8.t) : prop =
   forall (i:nat{i < Seq.length sc_all.g_size_classes}).
     within_size_class_i ptr (Seq.index (G.reveal sc_all.g_size_classes) i).data
-
-#restart-solver
 
 #push-options "--fuel 0 --ifuel 0 --z3rlimit 50"
 let mod_lt (a b: US.t)
@@ -276,79 +282,146 @@ let mod_lt (a b: US.t)
   = ()
 #pop-options
 
-inline_for_extraction noextract
-let u32_to_sz = Prelude.u32_to_sz
-
+open Prelude
 open Main
 
-inline_for_extraction noextract
-let slab_size = Main.sc_slab_region_size
-
 #push-options "--fuel 0 --ifuel 0 --z3rlimit 100 --query_stats"
-let slab_getsize ptr
+inline_for_extraction noextract
+val slab_getsize_aux_sc
+  (ptr: array U8.t)
+  (index: US.t)
+  (diff_sz: US.t)
+  (size: U32.t)
+  : Steel US.t
+  (A.varray ptr)
+  (fun _ -> A.varray ptr)
+  (requires fun h0 ->
+    US.v index < Seq.length sc_all.g_size_classes /\
+    (let sc : G.erased size_class = G.hide (Seq.index (G.reveal sc_all.g_size_classes) (US.v index)) in
+    let diff = A.offset (A.ptr_of ptr) - A.offset (A.ptr_of sc.data.slab_region) in
+    let size_as_union = TLA.get sizes index in
+    Sc? size_as_union /\
+    size == get_sc size_as_union /\
+    size == get_u32 size_as_union /\
+    size == get_u32 sc.data.size /\
+    US.v diff_sz == diff /\
+    same_base_array ptr sc.data.slab_region /\
+    0 <= diff /\
+    diff < US.v sc_slab_region_size /\
+    within_size_class_i ptr sc.data
+  ))
+  (ensures fun h0 result h1 ->
+    A.asel ptr h1 == A.asel ptr h0 /\
+    US.v result <= U32.v page_size /\
+    (let idx = sc_selection (US.sizet_to_uint32 result) in
+    (result <> 0sz ==> (
+      A.length ptr == U32.v size /\
+      (enable_slab_canaries_malloc ==>
+        A.length ptr == US.v result + 2
+      ) /\
+      (not enable_slab_canaries_malloc ==>
+        A.length ptr == US.v result
+      ) /\
+      (enable_sc_fast_selection ==>
+        A.length ptr == U32.v (get_u32 (L.index sc_list (US.v idx)))
+      )
+    ))
+  ))
+
+let slab_getsize_aux_sc ptr index diff_sz size
   =
-  //TODO: obviously false, will generate incorrect output
-  admit ();
-  SAA.within_bounds_elim
-    (A.split_l sc_all.slab_region 0sz)
-    (A.split_r sc_all.slab_region slab_region_size)
-    ptr;
-  UP.fits_lt
-    (A.offset (A.ptr_of ptr)
-    -
-    A.offset (A.ptr_of (A.split_l sc_all.slab_region 0sz)))
-    (US.v slab_region_size);
-  let diff = A.ptrdiff
-    ptr
-    (A.split_l sc_all.slab_region 0sz) in
-  let diff_sz = UP.ptrdifft_to_sizet diff in
-  let index = US.div diff_sz slab_size in
-  lemma_div_lt (US.v slab_size) (US.v nb_size_classes) (US.v nb_arenas) (US.v diff_sz);
-  total_nb_sc_lemma ();
-  assert (US.v index < US.v nb_size_classes * US.v nb_arenas);
-  assert (TLA.length sizes == US.v nb_size_classes * US.v nb_arenas);
-  assert (US.v index < TLA.length sizes);
-  let size = get_u32 (TLA.get sizes index) in
-  sizes_t_pred_elim sizes;
-  let index' = G.hide (US.v index % US.v nb_size_classes) in
-  assert (size = get_u32 (L.index sc_list index'));
-  if enable_sc_fast_selection then (
-    sc_selection_is_exact1 index';
-    sc_selection_is_exact2 index';
-    let index'' = G.hide (sc_selection size) in
-    assert (L.index sc_list (G.reveal index') == L.index sc_list (US.v (G.reveal index'')));
-    assert (size = get_u32 (L.index sc_list (US.v (G.reveal index''))))
-  ) else ();
-  let rem_slab = US.rem diff_sz slab_size in
-  let rem_slot = US.rem diff_sz (u32_to_sz page_size) in
-  // TODO: some refactor needed wrt SlotsFree
-  if US.rem rem_slot (US.uint32_to_sizet size) = 0sz then (
-    (**) let sc : G.erased size_class = G.hide (Seq.index (G.reveal sc_all.g_size_classes) (US.v index)) in
-    assert (size_class_pred sc_all.slab_region (G.reveal sc) (US.v index));
-    assert (A.offset (A.ptr_of (G.reveal sc).data.slab_region) == A.offset (A.ptr_of sc_all.slab_region) + (US.v index) * (US.v slab_size));
-    assert (US.v rem_slab == A.offset (A.ptr_of ptr) - A.offset (A.ptr_of (G.reveal sc).data.slab_region));
-    mod_lt diff_sz slab_size;
-    assert (US.v rem_slab < US.v slab_size);
-    mod_lt diff_sz (u32_to_sz page_size);
-    assert (US.v rem_slot == (A.offset (A.ptr_of ptr) - A.offset (A.ptr_of sc_all.slab_region)) % (U32.v page_size));
-    mod_lt rem_slot (US.uint32_to_sizet size);
+  (**) let sc : G.erased size_class = G.hide (Seq.index (G.reveal sc_all.g_size_classes) (US.v index)) in
+  assert (size_class_pred sc_all.slab_region (G.reveal sc) (US.v index));
+  // reveal synced_sizes
+  assume (not sc.data.is_extended);
+  let rem_page = US.rem diff_sz (u32_to_sz page_size) in
+  assert (US.v rem_page == (A.offset (A.ptr_of ptr) - A.offset (A.ptr_of sc.data.slab_region)) % (U32.v page_size));
+  if US.rem rem_page (u32_to_sz size) = 0sz then (
     (**) elim_within_size_class_i ptr (US.v index) size;
     (**) assert (A.length ptr == U32.v size);
+    let index' = G.hide (US.v index % US.v nb_size_classes) in
+    sizes_t_pred_elim sizes;
+    assert (size = get_u32 (L.index sc_list index'));
+    if enable_sc_fast_selection then (
+      sc_selection_is_exact1 index';
+      sc_selection_is_exact2 index'
+    ) else ();
     if enable_slab_canaries_malloc then
       return (US.uint32_to_sizet (size `U32.sub` 2ul))
     else
       return (US.uint32_to_sizet size)
   ) else (
-    // invalid pointer
     return 0sz
   )
 
-#restart-solver
+inline_for_extraction noextract
+val slab_getsize_aux_sc_ex
+  (ptr: array U8.t)
+  (index: US.t)
+  (diff_sz: US.t)
+  (size: U32.t)
+  : Steel US.t
+  (A.varray ptr)
+  (fun _ -> A.varray ptr)
+  (requires fun h0 ->
+    US.v index < Seq.length sc_all.g_size_classes /\
+    (let sc : G.erased size_class = G.hide (Seq.index (G.reveal sc_all.g_size_classes) (US.v index)) in
+    let diff = A.offset (A.ptr_of ptr) - A.offset (A.ptr_of sc.data.slab_region) in
+    let size_as_union = TLA.get sizes index in
+    Sc_ex? size_as_union /\
+    size == get_sc_ex size_as_union /\
+    size == get_u32 size_as_union /\
+    size == get_u32 sc.data.size /\
+    US.v diff_sz == diff /\
+    same_base_array ptr sc.data.slab_region /\
+    0 <= diff /\
+    diff < US.v sc_slab_region_size /\
+    within_size_class_i ptr sc.data
+  ))
+  (ensures fun h0 result h1 ->
+    A.asel ptr h1 == A.asel ptr h0 /\
+    US.v result <= max_sc_ex /\
+    (let idx = sc_selection (US.sizet_to_uint32 result) in
+    (result <> 0sz ==> (
+      A.length ptr == U32.v size /\
+      (enable_slab_canaries_malloc ==>
+        A.length ptr == US.v result + 2
+      ) /\
+      (not enable_slab_canaries_malloc ==>
+        A.length ptr == US.v result
+      ) /\
+      (enable_sc_fast_selection ==>
+        A.length ptr == U32.v (get_u32 (L.index sc_list (US.v idx)))
+      )
+    ))
+  ))
 
-let slab_free ptr
+let slab_getsize_aux_sc_ex ptr index diff_sz size
   =
-  //TODO: obviously false, will generate incorrect output
-  admit ();
+  (**) let sc : G.erased size_class = G.hide (Seq.index (G.reveal sc_all.g_size_classes) (US.v index)) in
+  assert (size_class_pred sc_all.slab_region (G.reveal sc) (US.v index));
+  // reveal synced_sizes
+  assume (sc.data.is_extended);
+  if US.rem diff_sz sc_ex_slab_size = 0sz then (
+    (**) elim_within_size_class_i ptr (US.v index) size;
+    (**) assert (A.length ptr == U32.v size);
+    let index' = G.hide (US.v index % US.v nb_size_classes) in
+    sizes_t_pred_elim sizes;
+    assert (size = get_u32 (L.index sc_list index'));
+    if enable_sc_fast_selection then (
+      sc_selection_is_exact1 index';
+      sc_selection_is_exact2 index'
+    ) else ();
+    if enable_slab_canaries_malloc then
+      return (US.uint32_to_sizet (size `U32.sub` 2ul))
+    else
+      return (US.uint32_to_sizet size)
+  ) else (
+    return 0sz
+  )
+
+let slab_getsize ptr
+  =
   SAA.within_bounds_elim
     (A.split_l sc_all.slab_region 0sz)
     (A.split_r sc_all.slab_region slab_region_size)
@@ -362,26 +435,76 @@ let slab_free ptr
     ptr
     (A.split_l sc_all.slab_region 0sz) in
   let diff_sz = UP.ptrdifft_to_sizet diff in
-  let index = US.div diff_sz slab_size in
-  lemma_div_lt (US.v slab_size) (US.v nb_size_classes) (US.v nb_arenas) (US.v diff_sz);
+  let index = US.div diff_sz sc_slab_region_size in
+  lemma_div_lt (US.v sc_slab_region_size) (US.v nb_size_classes) (US.v nb_arenas) (US.v diff_sz);
   total_nb_sc_lemma ();
-  assert (US.v index < US.v nb_size_classes * US.v nb_arenas);
-  assert (TLA.length sizes == US.v nb_size_classes * US.v nb_arenas);
-  assert (US.v index < TLA.length sizes);
-  let size = get_u32 (TLA.get sizes index) in
-  let rem_slab = US.rem diff_sz slab_size in
-  let rem_slot = US.rem diff_sz (u32_to_sz page_size) in
-  // TODO: some refactor needed wrt SlotsFree
-  if US.rem rem_slot (US.uint32_to_sizet size) = 0sz then (
-    (**) let sc = G.hide (Seq.index (G.reveal sc_all.g_size_classes) (US.v index)) in
-    assert (size_class_pred sc_all.slab_region (G.reveal sc) (US.v index));
-    assert (A.offset (A.ptr_of (G.reveal sc).data.slab_region) == A.offset (A.ptr_of sc_all.slab_region) + (US.v index) * (US.v slab_size));
-    assert (US.v rem_slab == A.offset (A.ptr_of ptr) - A.offset (A.ptr_of (G.reveal sc).data.slab_region));
-    mod_lt diff_sz slab_size;
-    assert (US.v rem_slab < US.v slab_size);
-    mod_lt diff_sz (u32_to_sz page_size);
-    assert (US.v rem_slot == (A.offset (A.ptr_of ptr) - A.offset (A.ptr_of sc_all.slab_region)) % (U32.v page_size));
-    mod_lt rem_slot (US.uint32_to_sizet size);
+  assert (US.v index < total_nb_sc);
+  mod_lt index nb_size_classes;
+  let size_as_union = TLA.get sizes index in
+  let size = get_u32 size_as_union in
+
+  (**) let sc : G.erased size_class = G.hide (Seq.index (G.reveal sc_all.g_size_classes) (US.v index)) in
+  // reveal size_class_pred
+  assume (A.offset (A.ptr_of (G.reveal sc).data.slab_region) == A.offset (A.ptr_of sc_all.slab_region) + US.v index * US.v sc_slab_region_size);
+
+  let rem_sc = US.rem diff_sz sc_slab_region_size in
+  assert (US.v rem_sc == A.offset (A.ptr_of ptr) - A.offset (A.ptr_of (G.reveal sc).data.slab_region));
+
+  assume (size == get_u32 sc.data.size);
+  assume (same_base_array ptr sc.data.slab_region);
+  if Sc? size_as_union then
+    slab_getsize_aux_sc ptr index rem_sc size
+  else
+    slab_getsize_aux_sc_ex ptr index rem_sc size
+
+#restart-solver
+
+#restart-solver
+
+inline_for_extraction noextract
+val slab_free_aux_sc
+  (ptr: array U8.t)
+  (index: US.t)
+  (diff_sz: US.t)
+  (size: U32.t)
+  : Steel bool
+  (A.varray ptr)
+  (fun b -> if b then emp else A.varray ptr)
+  (requires fun h0 ->
+    Seq.length sc_all.g_size_classes == US.v nb_size_classes * US.v nb_arenas /\
+    US.v index < Seq.length sc_all.g_size_classes /\
+    (let sc : G.erased size_class = G.hide (Seq.index (G.reveal sc_all.g_size_classes) (US.v index)) in
+    let diff = A.offset (A.ptr_of ptr) - A.offset (A.ptr_of sc.data.slab_region) in
+    let size_as_union = TLA.get sizes index in
+    Sc? size_as_union /\
+    size == get_sc size_as_union /\
+    size == get_u32 size_as_union /\
+    size == get_u32 sc.data.size /\
+    US.v diff_sz == diff /\
+    same_base_array ptr sc.data.slab_region /\
+    0 <= diff /\
+    diff < US.v sc_slab_region_size /\
+    within_size_class_i ptr sc.data
+  ))
+  (ensures fun h0 r _ ->
+    let s = A.asel ptr h0 in
+    enable_slab_canaries_free ==>
+      (r ==>
+        A.length ptr >= 2 /\
+        Seq.index s (A.length ptr - 2) == slab_canaries_magic1 /\
+        Seq.index s (A.length ptr - 1) == slab_canaries_magic2
+      )
+  )
+
+let slab_free_aux_sc ptr index diff_sz size
+  =
+  (**) let sc : G.erased size_class = G.hide (Seq.index (G.reveal sc_all.g_size_classes) (US.v index)) in
+  assert (size_class_pred sc_all.slab_region (G.reveal sc) (US.v index));
+  // reveal synced_sizes
+  assume (not sc.data.is_extended);
+  let rem_page = US.rem diff_sz (u32_to_sz page_size) in
+  assert (US.v rem_page == (A.offset (A.ptr_of ptr) - A.offset (A.ptr_of sc.data.slab_region)) % (U32.v page_size));
+  if US.rem rem_page (u32_to_sz size) = 0sz then (
     (**) elim_within_size_class_i ptr (US.v index) size;
     (**) assert (A.length ptr == U32.v size);
     if enable_slab_canaries_free then (
@@ -389,15 +512,111 @@ let slab_free ptr
       let magic1 = A.index ptr (US.uint32_to_sizet (size `U32.sub` 2ul)) in
       let magic2 = A.index ptr (US.uint32_to_sizet (size `U32.sub` 1ul)) in
       if magic1 = slab_canaries_magic1 && magic2 = slab_canaries_magic2 then
-        slab_free' index ptr rem_slab
+        slab_free' index ptr diff_sz
       else
         // Canary was overwritten
         return false
     ) else (
-      slab_free' index ptr rem_slab
+      slab_free' index ptr diff_sz
     )
   ) else (
     return false
   )
-#pop-options
+
+inline_for_extraction noextract
+val slab_free_aux_sc_ex
+  (ptr: array U8.t)
+  (index: US.t)
+  (diff_sz: US.t)
+  (size: U32.t)
+  : Steel bool
+  (A.varray ptr)
+  (fun b -> if b then emp else A.varray ptr)
+  (requires fun h0 ->
+    Seq.length sc_all.g_size_classes == US.v nb_size_classes * US.v nb_arenas /\
+    US.v index < Seq.length sc_all.g_size_classes /\
+    (let sc : G.erased size_class = G.hide (Seq.index (G.reveal sc_all.g_size_classes) (US.v index)) in
+    let diff = A.offset (A.ptr_of ptr) - A.offset (A.ptr_of sc.data.slab_region) in
+    let size_as_union = TLA.get sizes index in
+    Sc_ex? size_as_union /\
+    size == get_sc_ex size_as_union /\
+    size == get_u32 size_as_union /\
+    size == get_u32 sc.data.size /\
+    US.v diff_sz == diff /\
+    same_base_array ptr sc.data.slab_region /\
+    0 <= diff /\
+    diff < US.v sc_slab_region_size /\
+    within_size_class_i ptr sc.data
+  ))
+  (ensures fun h0 r _ ->
+    let s = A.asel ptr h0 in
+    enable_slab_canaries_free ==>
+      (r ==>
+        A.length ptr >= 2 /\
+        Seq.index s (A.length ptr - 2) == slab_canaries_magic1 /\
+        Seq.index s (A.length ptr - 1) == slab_canaries_magic2
+      )
+  )
+
+let slab_free_aux_sc_ex ptr index diff_sz size
+  =
+  (**) let sc : G.erased size_class = G.hide (Seq.index (G.reveal sc_all.g_size_classes) (US.v index)) in
+  assert (size_class_pred sc_all.slab_region (G.reveal sc) (US.v index));
+  // reveal synced_sizes
+  assume (sc.data.is_extended);
+  if US.rem diff_sz sc_ex_slab_size = 0sz then (
+    if enable_slab_canaries_free then (
+      enable_slab_canaries_lemma ();
+      let magic1 = A.index ptr (US.uint32_to_sizet (size `U32.sub` 2ul)) in
+      let magic2 = A.index ptr (US.uint32_to_sizet (size `U32.sub` 1ul)) in
+      if magic1 = slab_canaries_magic1 && magic2 = slab_canaries_magic2 then
+        slab_free' index ptr diff_sz
+      else
+        // Canary was overwritten
+        return false
+    ) else (
+      slab_free' index ptr diff_sz
+    )
+  ) else (
+    return false
+  )
+
+let slab_free ptr
+  =
+  SAA.within_bounds_elim
+    (A.split_l sc_all.slab_region 0sz)
+    (A.split_r sc_all.slab_region slab_region_size)
+    ptr;
+  UP.fits_lt
+    (A.offset (A.ptr_of ptr)
+    -
+    A.offset (A.ptr_of (A.split_l sc_all.slab_region 0sz)))
+    (US.v slab_region_size);
+  let diff = A.ptrdiff
+    ptr
+    (A.split_l sc_all.slab_region 0sz) in
+  let diff_sz = UP.ptrdifft_to_sizet diff in
+  let index = US.div diff_sz sc_slab_region_size in
+  lemma_div_lt (US.v sc_slab_region_size) (US.v nb_size_classes) (US.v nb_arenas) (US.v diff_sz);
+  total_nb_sc_lemma ();
+  assert (US.v index < total_nb_sc);
+  mod_lt index nb_size_classes;
+  let size_as_union = TLA.get sizes index in
+  let size = get_u32 size_as_union in
+
+  (**) let sc : G.erased size_class = G.hide (Seq.index (G.reveal sc_all.g_size_classes) (US.v index)) in
+  // reveal size_class_pred
+  assume (A.offset (A.ptr_of (G.reveal sc).data.slab_region) == A.offset (A.ptr_of sc_all.slab_region) + US.v index * US.v sc_slab_region_size);
+
+  let rem_sc = US.rem diff_sz sc_slab_region_size in
+  assert (US.v rem_sc == A.offset (A.ptr_of ptr) - A.offset (A.ptr_of (G.reveal sc).data.slab_region));
+
+  assume (size == get_u32 sc.data.size);
+  assume (same_base_array ptr sc.data.slab_region);
+  assume (U32.v size > 0);
+
+  if Sc? size_as_union then
+    slab_free_aux_sc ptr index rem_sc size
+  else
+    slab_free_aux_sc_ex ptr index rem_sc size
 
